data/validation/proofs/Tree.v
@@ -11,19 +11,23 @@ Inductive Tree : Type :=
 
 Inductive depth : Tree -> nat -> Prop :=
 | depth_leaf : depth Leaf 0
-| depth_node : forall v l r n,
-  depth l n -> depth r n ->
-  depth (Node l v r) (n + 1).
+| depth_node : forall v l r n n1 n2,
+  depth l n1 -> depth r n2 ->
+  n = (max n1 n2) ->
+  depth (Node l v r) (S n).
 
 Inductive complete : Tree -> Prop :=
 | CompleteLeaf :
 complete Leaf
 | CompleteNode : forall n x l r,
-complete l -> complete r -> depth l n -> depth r n ->
+complete l -> complete r -> depth l n -> depth r n -> depth (Node l x r) (S n) ->
 complete (Node l x r).
 
 Inductive leaf : Tree -> Prop :=
 | leaf_i : leaf Leaf.
+
+Inductive root : Tree -> nat -> Prop :=
+| root_i : forall l v r, root (Node l v r) v.
 
 Inductive lch : Tree -> Tree -> Prop :=
 | lch_i: forall v l r, lch (Node l v r) l.
@@ -31,12 +35,22 @@ Inductive lch : Tree -> Tree -> Prop :=
 Inductive rch  : Tree -> Tree  -> Prop :=
 | rch_i: forall v l r, rch (Node l v r) r.
 
+Inductive tree_mem : Tree -> nat -> Prop :=
+| BstNode_root : forall l v r, tree_mem (Node l v r) v
+| BstNode_child : forall l v c r, (tree_mem l c \/ tree_mem r c) -> tree_mem (Node l v r) c.
+
+Inductive bst : Tree -> Prop :=
+| BstLeaf : bst Leaf
+| BstNode : forall x l r, (forall lo, tree_mem l lo -> lo < x) -> (forall hi, tree_mem r hi -> x < hi) -> bst l -> bst r -> bst (Node l x r).
+
 Hint Constructors leaf: core.
-(* Hint Constructors root: core. *)
+Hint Constructors root: core.
 Hint Constructors lch: core.
 Hint Constructors rch: core.
 Hint Constructors depth: core.
 Hint Constructors complete: core.
+Hint Constructors tree_mem: core.
+Hint Constructors bst: core.
 Hint Unfold not: core.
 
 Lemma tree_complete_leaf : forall l, (leaf l -> complete l). Proof.
@@ -50,13 +64,13 @@ Lemma tree_depth_leaf : forall l, (leaf l -> depth l 0). Proof.
 Lemma tree_complete_node : forall l, (forall l1, (forall l2, (forall n, ((complete l1 /\ (complete l2 /\ (depth l1 n /\ (depth l2 n /\ (lch l l1 /\ rch l l2))))) -> complete l)))). Proof.
 intros. simp. destruct l.
     - constructor.
-    - my_inversion H3; clear H3. my_inversion H4; clear H4. econstructor; eauto.
+    - my_inversion H3; clear H3. my_inversion H4; clear H4. econstructor; eauto. econstructor; eauto. lia.
  Qed. Hint Resolve tree_complete_node: core.
 
 Lemma tree_depth_node : forall l, (forall l1, (forall l2, (forall n, ((depth l1 n /\ (depth l2 n /\ (lch l l1 /\ rch l l2))) -> depth l (n + 1))))). Proof.
     intros. simp. destruct l.
     - my_inversion H1.
-    - my_inversion H1; clear H1. my_inversion H2; clear H2. constructor; auto.
+    - my_inversion H1; clear H1. my_inversion H2; clear H2. assert (n + 1 = S n). lia. rewrite H1. econstructor; eauto. lia.
  Qed. Hint Resolve tree_depth_node: core.
 
 Lemma tree_complete_lch_complete : forall l, (forall l1, ((lch l l1 /\ complete l) -> complete l1)). Proof.
@@ -67,10 +81,155 @@ Lemma tree_complete_rch_complete : forall l, (forall l1, ((rch l l1 /\ complete 
     intros. simp. my_inversion H0. my_inversion H. my_inversion H.
  Qed. Hint Resolve tree_complete_rch_complete: core.
 
-Lemma tree_complete_lch_depth_minus_1 : forall l, (forall l1, (forall n, ((lch l l1 /\ (complete l /\ depth l n)) -> depth l1 (n - 1)))). Proof.
-    intros. simp. my_inversion H1; clear H1. my_inversion H. my_inversion H; clear H. assert (n0 + 1 - 1 = n0). lia. rewrite H. auto.
- Qed. Hint Resolve tree_complete_lch_depth_minus_1: core.
+Lemma max_helper : forall n1 n2, 0 = Nat.max n1 n2 -> (n1 = 0 /\ n2 = 0). Proof.
+    intros. destruct n1; destruct n2; auto. my_inversion H.
+Qed.
 
-Lemma tree_complete_rch_depth_minus_1 : forall l, (forall l1, (forall n, ((rch l l1 /\ (complete l /\ depth l n)) -> depth l1 (n - 1)))). Proof.
-    intros. simp. my_inversion H1; clear H1. my_inversion H. my_inversion H; clear H. assert (n0 + 1 - 1 = n0). lia. rewrite H. auto.
- Qed. Hint Resolve tree_complete_rch_depth_minus_1: core.
+Lemma max_helper2 : forall n n1 n2, n = Nat.max n1 n2 -> (n1 = n \/ n2 = n). Proof.
+    intros. destruct n1; destruct n2; auto. my_inversion H. simp.
+    apply PeanoNat.Nat.max_case. left; auto. right; auto.
+Qed.
+
+Lemma max_helper3 : forall n1 n2, (n1 = Nat.max n1 n2 \/ n2 = Nat.max n1 n2). Proof.
+    intros.
+    apply PeanoNat.Nat.max_case. left; auto. right; auto.
+Qed.
+
+Lemma depth_helper : forall t n1 n2, depth t n1 -> depth t n2 -> n1 = n2.
+Proof.
+    induction t; simpl; intros.
+    + inversion H. inversion H0. reflexivity.
+    + inversion H; subst. inversion H0; subst.
+      specialize IHt2 with n3 n4.
+      specialize IHt1 with n0 n1.
+      apply IHt1 in H4.
+      - subst. apply IHt2 in H6.
+      * subst. reflexivity.
+      * assumption.
+      - assumption.
+Qed.
+
+Lemma tree_complete_lch_depth_minus_1 : forall l, (forall l1, (forall n, ((lch l l1 /\ (complete l /\ depth l n)) -> depth l1 (n - 1)))). Proof.
+    intros. simp. destruct l.
+    - my_inversion H.
+    - my_inversion H0. my_inversion H; clear H. my_inversion H1. apply PeanoNat.Nat.max_case.
+        + assert (S n2 - 1 = n2); try lia. rewrite H; auto.
+        + assert (S n3 - 1 = n3); try lia. rewrite H. assert (n3 = n0).
+            * eapply depth_helper; eauto.
+            * subst; auto.
+Qed. Hint Resolve tree_complete_lch_depth_minus_1: core.
+
+Lemma tree_complete_rch_depth_minus_1 : forall l, (forall l1, (forall n, ((rch l l1 /\ (complete l /\ depth l n)) -> depth l1 (n - 1)))).
+Proof.
+    intros. simp. destruct l.
+    - my_inversion H.
+    - my_inversion H0. my_inversion H; clear H. my_inversion H1. apply PeanoNat.Nat.max_case.
+        + assert (S n2 - 1 = n2); try lia. rewrite H. assert (n2 = n0).
+            * eapply depth_helper; eauto.
+            * subst; auto.
+        + assert (S n3 - 1 = n3); try lia. rewrite H; auto.
+Qed. Hint Resolve tree_complete_rch_depth_minus_1: core.
+
+ Lemma tree_leaf_bst : forall l, (leaf l -> bst l). Proof.
+    intros. my_inversion H. constructor.
+  Qed. Hint Resolve tree_leaf_bst: core.
+
+Lemma tree_bst_lch_bst : forall l, (forall l1, ((lch l l1 /\ bst l) -> bst l1)). Proof.
+    intros. simp. my_inversion H0.
+    - my_inversion H.
+    - my_inversion H.
+ Qed. Hint Resolve tree_bst_lch_bst: core.
+
+Lemma tree_bst_rch_bst : forall l, (forall l1, ((rch l l1 /\ bst l) -> bst l1)). Proof.
+    intros. simp. my_inversion H0.
+    - my_inversion H.
+    - my_inversion H.
+ Qed. Hint Resolve tree_bst_rch_bst: core.
+
+Lemma tree_bst_lch_mem_lt_root : forall l, (forall l1, (forall x, (forall y, ((bst l /\ (lch l l1 /\ (root l x /\ tree_mem l1 y))) -> y < x)))). Proof.
+    intros. simp.
+    - my_inversion H.
+        + my_inversion H1.
+        + my_inversion H1; clear H1. my_inversion H0; clear H0. apply H3. auto.
+ Qed. Hint Resolve tree_bst_lch_mem_lt_root: core.
+
+Lemma tree_bst_rch_mem_gt_root : forall l, (forall l1, (forall x, (forall y, ((bst l /\ (rch l l1 /\ (root l x /\ tree_mem l1 y))) -> x < y)))). Proof.
+        intros. simp.
+    - my_inversion H.
+        + my_inversion H1.
+        + my_inversion H1; clear H1. my_inversion H0; clear H0. apply H4. auto.
+ Qed. Hint Resolve tree_bst_rch_mem_gt_root: core.
+
+ Lemma tree_root_mem : forall l, (forall x, (root l x -> tree_mem l x)). Proof.
+    intros. my_inversion H. auto.
+  Qed. Hint Resolve tree_root_mem: core.
+
+Lemma tree_mem_lch_mem : forall l, (forall l1, (forall x, ((lch l l1 /\ tree_mem l1 x) -> tree_mem l x))). Proof.
+    intros. simp. my_inversion H; clear H. auto.
+Qed. Hint Resolve tree_mem_lch_mem: core.
+
+Lemma tree_mem_rch_mem : forall l, (forall l1, (forall x, ((rch l l1 /\ tree_mem l1 x) -> tree_mem l x))). Proof.
+    intros. simp. my_inversion H. auto.
+ Qed. Hint Resolve tree_mem_rch_mem: core.
+
+Lemma tree_leaf_no_root : forall l, (forall x, (leaf l -> ~root l x)). Proof.
+    intros. my_inversion H. unfold not. intro. my_inversion H0.
+ Qed. Hint Resolve tree_leaf_no_root: core.
+
+Lemma tree_leaf_no_ch : forall l, (forall l1, (leaf l -> ~(lch l l1 \/ rch l l1))). Proof.
+    intros. unfold not; intro. my_inversion H. my_inversion H0; my_inversion H1.
+ Qed. Hint Resolve tree_leaf_no_ch: core.
+
+Lemma tree_no_leaf_exists_ch : forall l, (exists l1, (exists l2, (~leaf l -> (lch l l1 /\ rch l l2)))). Proof.
+    intros. destruct l; repeat econstructor.
+    - destruct H; constructor. Unshelve. constructor. constructor.
+    - destruct H; constructor.
+ Qed. Hint Resolve tree_no_leaf_exists_ch: core.
+
+Lemma tree_no_leaf_exists_root : forall l, (exists x, (~leaf l -> root l x)). Proof.
+    intros. destruct l; repeat econstructor. intro. destruct H. constructor. Unshelve. constructor.
+ Qed. Hint Resolve tree_no_leaf_exists_root: core.
+
+Lemma tree_root_no_leaf : forall l, (forall x, (root l x -> ~leaf l)). Proof.
+    - intros. my_inversion H. unfold not. intros. my_inversion H0.
+ Qed. Hint Resolve tree_root_no_leaf: core.
+
+Lemma tree_ch_no_leaf : forall l, (forall l1, ((lch l l1 \/ rch l l1) -> ~leaf l)). Proof.
+    intros. my_inversion H; clear H; unfold not; intro; my_inversion H0; my_inversion H.
+Qed. Hint Resolve tree_ch_no_leaf: core.
+
+Lemma tree_depth_geq_0 : forall l, (forall n, (depth l n -> n >= 0)). Proof.
+    intros. lia.
+ Qed. Hint Resolve tree_depth_geq_0: core.
+
+Lemma tree_leaf_depth_0 : forall l, (forall n, ((leaf l /\ depth l n) -> n = 0)). Proof.
+    intros. simp. my_inversion H. my_inversion H0.
+ Qed. Hint Resolve tree_leaf_depth_0: core.
+
+Lemma tree_positive_depth_is_not_leaf : forall l, (forall n, ((depth l n /\ n > 0) -> ~leaf l)). Proof.
+    intros. simp. unfold not. intro. my_inversion H1. my_inversion H. my_inversion H0.
+ Qed. Hint Resolve tree_positive_depth_is_not_leaf: core.
+
+Lemma tree_depth_exists : forall l, exists n, depth l n.
+Proof.
+    intro. induction l.
+    - exists 0. constructor.
+    - my_inversion IHl1. my_inversion IHl2. exists (S (max x x0)). econstructor; eauto.
+Qed.
+
+Lemma tree_ch_depth_ex : forall l, (forall l1, (forall n, (exists n1, (((lch l l1 \/ rch l l1) /\ depth l n) -> depth l1 n1)))). Proof.
+    intros. assert (exists n', depth l1 n'). apply tree_depth_exists. destruct H. exists x. intro. auto.
+Qed. Hint Resolve tree_ch_depth_ex: core.
+
+
+Lemma tree_ch_depth_minus_1 : forall l, (forall l1, (forall n, (forall n1, (((lch l l1 \/ rch l l1) /\ (depth l n /\ depth l1 n1)) -> n1 <= (n - 1))))).
+Proof.
+    intros. simp. my_inversion H0.
+    - destruct H; my_inversion H.
+    - destruct H; my_inversion H; clear H. assert (n1 = n2). eapply depth_helper; eauto. lia. assert (n1 = n3). eapply depth_helper; eauto. lia.
+Qed.
+Hint Resolve tree_ch_depth_minus_1: core.
+
+Lemma tree_depth_0_is_leaf : forall l, (forall n, ((depth l n /\ n = 0) -> leaf l)). Proof.
+    intros. simp. my_inversion H. constructor.
+Qed. Hint Resolve tree_depth_0_is_leaf: core.
